engines/thales/Js.lean
@@ -1,0 +1,5 @@
+import Js.NormAttr
+import Js.Runtime
+import Js.Number.Basic
+import Js.Number.FloatOps
+import Js.Number.FloatFacts
